Examples/Parser_Test/Parser_Test.thy
@@ -25,9 +25,26 @@ lemma "parser_test_firewall \<equiv>
             (MatchAnd (Match (Dst_Ports [(1, 0xFFFF)]))
               (Match (Extra ''--tcp-flags FIN,SYN,RST,ACK SYN'')))))
     action.Accept,
-   Rule (Match (Prot (Proto UDP))) Return, Rule (Match (Prot (Proto ICMP))) action.Accept]),
+   Rule (Match (Prot (Proto UDP))) Return,
+   Rule (MatchAnd (Match (Prot (Proto ICMP))) (Match (Extra ''-m icmp --icmp-type 3/4'')))
+    action.Accept,
+   Rule (MatchAnd (Match (Prot (Proto ICMP)))
+          (Match (Extra [CHR ''-'', CHR ''m'', CHR '' '', CHR ''c'', CHR ''o'', CHR ''m'', CHR ''m'',
+                         CHR ''e'', CHR ''n'', CHR ''t'', CHR '' '', CHR ''-'', CHR ''-'', CHR ''c'',
+                         CHR ''o'', CHR ''m'', CHR ''m'', CHR ''e'', CHR ''n'', CHR ''t'', CHR '' '',
+                         Char Nibble2 Nibble2, CHR ''!'', Char Nibble2 Nibble2])))
+    action.Accept,
+   Rule (Match (Prot (Proto ICMP))) action.Accept]),
  (''FORWARD'',
-  [Rule (Match (Src (Ip4AddrNetmask (127, 0, 0, 0) 8))) action.Drop,
+  [Rule (Match (Extra [CHR ''-'', CHR ''-'', CHR ''l'', CHR ''o'', CHR ''g'', CHR ''-'', CHR ''p'',
+                       CHR ''r'', CHR ''e'', CHR ''f'', CHR ''i'', CHR ''x'', CHR '' '',
+                       Char Nibble2 Nibble2, CHR ''!'', CHR ''#'', CHR ''*'', CHR ''~'', CHR ''%'',
+                       CHR ''&'', CHR ''/'', CHR ''('', CHR '')'', CHR ''='', CHR ''?'',
+                       Char Nibble2 Nibble2, CHR '' '', CHR ''-'', CHR ''-'', CHR ''l'', CHR ''o'',
+                       CHR ''g'', CHR ''-'', CHR ''l'', CHR ''e'', CHR ''v'', CHR ''e'', CHR ''l'',
+                       CHR '' '', CHR ''6'']))
+    Log,
+   Rule (Match (Src (Ip4AddrNetmask (127, 0, 0, 0) 8))) action.Drop,
    Rule (MatchAnd (Match (IIface (Iface ''wlan0'')))
           (MatchAnd (Match (Prot (Proto TCP)))
             (MatchAnd (Match (Extra ''-m tcp ! --tcp-flags FIN,SYN,RST,ACK SYN''))
@@ -35,16 +52,16 @@ lemma "parser_test_firewall \<equiv>
     action.Drop,
    Rule (Match (Extra ''-m conntrack --ctstate NEW,INVALID'')) action.Drop,
    Rule (MatchAnd (Match (IIface (Iface ''wlan0'')))
-          (MatchAnd (Match (Prot (Proto ICMP))) (Match (CT_State {CT_Established, CT_New}))))
+          (MatchAnd (Match (Prot (Proto ICMP)))
+            (Match (CT_State {CT_Established, CT_New, CT_Related, CT_Untracked}))))
     action.Accept,
    Rule (Match (CT_State {CT_New, CT_Untracked})) action.Accept,
-   Rule (Match (CT_State {CT_Established})) action.Accept,
+   Rule (Match (CT_State {CT_Established, CT_Related})) action.Accept,
    Rule (MatchNot (Match (IIface (Iface ''eth+'')))) action.Drop,
    Rule (MatchAnd (Match (Src (Ip4AddrNetmask (100, 0, 0, 0) 24))) (Match (Prot (Proto TCP))))
     (Call ''DOS~Pro-t_ect''),
    Rule (MatchNot (Match (Src (Ip4AddrNetmask (131, 159, 0, 0) 16)))) action.Drop,
-   Rule (MatchAnd (Match (Prot (Proto TCP))) (Match (Dst_Ports [(0x50, 0x50), (0x1BB, 0x1BB)])))
-    Return,
+   Rule (MatchAnd (Match (Prot (Proto TCP))) (Match (Dst_Ports [(0x50, 0x50), (0x1BB, 0x1BB)]))) Return,
    Rule (MatchAnd (Match (Dst (Ip4AddrNetmask (127, 0, 0, 1) 32)))
           (MatchAnd (Match (OIface (Iface ''eth1.152'')))
             (MatchAnd (Match (Prot (Proto UDP)))
@@ -59,6 +76,8 @@ lemma "parser_test_firewall \<equiv>
                      [(0x15, 0x15), (0x369, 0x36A), (0x138D, 0x138D), (0x138E, 0x138E), (0x50, 0x50),
                       (0x224, 0x224), (0x6F, 0x6F), (0x37C, 0x37C), (0x801, 0x801)]))))
     action.Drop,
+   Rule (Match (Src (Ip4AddrRange (127, 0, 0, 1) (127, 0, 10, 0)))) Return,
+   Rule (MatchNot (Match (Dst (Ip4AddrRange (127, 0, 0, 1) (127, 0, 10, 0))))) Return,
    Rule MatchAny (Goto ''Terminal'')]),
  (''INPUT'', []), (''OUTPUT'', []),
  (''Terminal'',
